new

Automata/Fin.lean
@@ -7,66 +7,86 @@ import Mathlib.Tactic
 #check Fin.castPred
 #check Fin.predAbove
 #check Fin.succAboveCases
+#check Fin.removeNth
 
 variable {α : Type} {n : ℕ}
 
 #check Fin.succAboveCases (α := (fun _ => α)) (n := n)
 
-def remove_index (i : Fin (n + 1)) (f: Fin (n + 1) → α) (j : Fin n) : α  := f (Fin.succAbove i j)
+def remove_index' (i : Fin (n + 1)) (f: Fin (n + 1) → α) (j : Fin n) : α  := f (Fin.succAbove i j)
 
-def Fin.insert (i : Fin (n + 1)) (a : α) (f : Fin n → α) (j : Fin (n + 1)) : α := Fin.succAboveCases i a f j
+def remove_index := @Fin.removeNth
 
+def Fin.insert' (i : Fin (n + 1)) (a : α) (f : Fin n → α) (j : Fin (n + 1)) : α := Fin.succAboveCases i a f j
+
+def Fin.insert := @Fin.insertNth
+
+#check Fin.insertNth
+
+section
+
+variable (i : Fin (n + 1)) (a : α) (f : Fin n → α) (j : Fin (n + 1))
+
+end
 def recover_index (i : Fin (n + 1)) (k: Fin n) (f: Fin n → α):
   (Fin (n + 1) → α) := Fin.insert i (f k) f
 
-def recover_value (i : Fin (n + 1)) (x: Fin (b+2)) (f: Fin n → Fin (b+2)) :
- (Fin (n + 1) → Fin (b+2)) := Fin.insert i x f
+
+def recover_value' (i : Fin (n + 1)) (x : α) (f: Fin n → α) :
+ (Fin (n + 1) → α) := Fin.insert i x f
+
+def recover_value := @Fin.insert
 
 @[simp] theorem remove_insert (i : Fin (n + 1)) (f: Fin n → α) :
   remove_index i (Fin.insert i a f) = f := by
   ext x
-  simp_all[remove_index, Fin.insert, Fin.succAboveCases, Fin.succAbove]
-  split; simp_all only [Fin.castPred_castSucc, dite_eq_ite, ite_eq_else]
-  . intro h
-    omega
-  . split
-    . rename_i h h'
-      simp_all [Fin.succ, Fin.castSucc, Fin.castAdd, Fin.castLE]
-      have : i.val ≤ x.val := by
-        -- Hard, need aesop
-        subst h'
-        simp_all only [Fin.mk_le_mk, add_le_iff_nonpos_right, nonpos_iff_eq_zero, one_ne_zero]
-      have : x.val + 1 = i := by
-        subst h'
-        simp_all only [Fin.mk_le_mk, add_le_iff_nonpos_right, nonpos_iff_eq_zero, one_ne_zero]
-      omega
-    . split; simp_all only [Fin.succ, Nat.succ_eq_add_one, Fin.castPred, Fin.castLT_mk]
-      . rename_i h h' h'''
-        have : x.val + 1 < i.val := by
-          simp_all only [not_lt]
-          exact h'
-        have : ¬ x.val < i := by
-          simp_all only [not_lt]
-          exact h
-        omega
-      . simp only [Fin.pred_succ]
+  -- simp_all[remove_index, Fin.insert, Fin.succAboveCases, Fin.succAbove, Fin.removeNth]
+  simp_all only [remove_index, Fin.removeNth, Fin.insert, Fin.succAbove_cases_eq_insertNth,
+    Fin.insertNth_apply_succAbove]
+
+
+  -- split; simp_all only [Fin.insertNth, Fin.succAboveCases, Fin.castPred_castSucc, dite_eq_ite, ite_eq_else, Fin.castSucc, Fin.castAdd, Fin.castLE, Fin.castPred, Fin.castLT]
+  -- . intro h
+  --   omega
+  -- . split
+  --   . rename_i h h'
+  --     simp_all [Fin.succ, Fin.castSucc, Fin.castAdd, Fin.castLE]
+  --     have : i.val ≤ x.val := by
+  --       -- Hard, need aesop
+  --       subst h'
+  --       simp_all only [Fin.mk_le_mk, add_le_iff_nonpos_right, nonpos_iff_eq_zero, one_ne_zero]
+  --     have : x.val + 1 = i := by
+  --       subst h'
+  --       simp_all only [Fin.mk_le_mk, add_le_iff_nonpos_right, nonpos_iff_eq_zero, one_ne_zero]
+  --     omega
+  --   . split; simp_all only [Fin.succ, Nat.succ_eq_add_one, Fin.castPred, Fin.castLT_mk]
+  --     . rename_i h h' h'''
+  --       have : x.val + 1 < i.val := by
+  --         simp_all only [not_lt]
+  --         exact h'
+  --       have : ¬ x.val < i := by
+  --         simp_all only [not_lt]
+  --         exact h
+  --       omega
+  --     . simp only [Fin.pred_succ]
 
 @[simp] theorem insert_remove (i : Fin (n + 1)) (a : α) (f: Fin (n + 1) → α) (hf: f i = a) :
   Fin.insert i a (remove_index i f) = f := by
   -- rw[remove_index]
   ext x
-  simp_all[remove_index, Fin.insert, Fin.succAboveCases, Fin.succAbove]
-  split
-  .
-    rename_i h
-    subst hf h
-    rfl
-  . split
-    . subst hf
-      rfl
-    . split <;> simp_all only [Fin.castSucc, Fin.castAdd, Fin.castLE, Fin.pred, Fin.coe_subNat]
-      . have: x.val - 1 < i.val := by
-          rename_i h_2
-          subst hf
-          exact h_2
-        omega
+  simp_all[remove_index, Fin.insert, Fin.succAboveCases, Fin.succAbove, Fin.removeNth,Function.update]
+
+  -- split
+  -- .
+  --   rename_i h
+  --   subst hf h
+  --   rfl
+  -- . split
+  --   . subst hf
+  --     rfl
+  --   . split <;> simp_all only [Fin.castSucc, Fin.castAdd, Fin.castLE, Fin.pred, Fin.coe_subNat]
+  --     . have: x.val - 1 < i.val := by
+  --         rename_i h_2
+  --         subst hf
+  --         exact h_2
+  --       omega
