Automata/Projection.lean
@@ -19,20 +19,19 @@ def project (m : Fin (n+1)) (dfa : DFA (Fin (n+1) → Fin (b+2)) state) [Decidab
   output := dfa.output
 }
 
-theorem project_transition [DecidableEq state](dfa : DFA (Fin (n + 1) → Fin (b+2)) state) (m : Fin (n + 1)) (f : (Fin (n+1) → Fin (b+2))) (p q : state) : dfa.transition f p = q → q ∈ ((project m dfa).transition (remove_index m f) p).val := by
+-- theorem transition_project' [DecidableEq state](dfa : DFA (Fin (n + 1) → Fin (b+2)) state) (m : Fin (n + 1)) (f : (Fin (n+1) → Fin (b+2))) (p q : state) : dfa.transition f p = q → q ∈ ((project m dfa).transition (remove_index m f) p).val := by
+--   simp only [project, List.mem_dedup, List.mem_map, FinEnum.mem_toList, true_and]
+--   intro h
+--   use f m
+--   simp[recover_value, insert_remove]
+--   exact h
+
+theorem transition_project [DecidableEq state](dfa : DFA (Fin (n + 1) → Fin (b+2)) state) (m : Fin (n + 1)) (f : (Fin (n+1) → Fin (b+2))) (p : state) : dfa.transition f p ∈ ((project m dfa).transition (remove_index m f) p).val := by
   simp only [project, List.mem_dedup, List.mem_map, FinEnum.mem_toList, true_and]
-  intro h
   use f m
   simp[recover_value, insert_remove]
-  exact h
 
-theorem project_transition' [DecidableEq state](dfa : DFA (Fin (n + 1) → Fin (b+2)) state) (m : Fin (n + 1)) (f : (Fin (n+1) → Fin (b+2))) (p : state) : dfa.transition f p ∈ ((project m dfa).transition (remove_index m f) p).val := by
-  simp only [project, List.mem_dedup, List.mem_map, FinEnum.mem_toList, true_and]
-  use f m
-  simp[recover_value, insert_remove]
-
-
-theorem project_transFrom [DecidableEq state](dfa : DFA (Fin (n + 1) → Fin (b+2)) state) (m : Fin (n + 1)) (l : List (Fin (n+1) → Fin (b+2))) (p q : state) : dfa.transFrom l p = q → q ∈ ((project m dfa).transFrom (l.map (fun f => remove_index m f)) ⟨[p], by exact List.nodup_singleton p⟩).val := by
+theorem transFrom_project [DecidableEq state](dfa : DFA (Fin (n + 1) → Fin (b+2)) state) (m : Fin (n + 1)) (l : List (Fin (n+1) → Fin (b+2))) (p q : state) : dfa.transFrom l p = q → q ∈ ((project m dfa).transFrom (l.map (fun f => remove_index m f)) ⟨[p], by exact List.nodup_singleton p⟩).val := by
   intro h
   induction l generalizing p
   case nil =>
@@ -47,25 +46,121 @@ theorem project_transFrom [DecidableEq state](dfa : DFA (Fin (n + 1) → Fin (b+
     have := NFA.transFrom_sublist (ps := ⟨[dfa.transition f p], by exact List.nodup_singleton (dfa.transition f p)⟩) (project m dfa) (List.map (fun f ↦ remove_index m f) fs) ⟨(((project m dfa).transition (remove_index m f) p).val).dedup, by apply List.nodup_dedup⟩
     apply this
     . simp only [List.cons_subset, List.mem_dedup, List.nil_subset, and_true]
-      apply project_transition'
+      apply transition_project
     . assumption
 
-theorem project_evalFrom [DecidableEq state](dfa : DFA (Fin (n + 1) → Fin (b+2)) state) (m : Fin (n + 1)) (l : List (Fin (n+1) → Fin (b+2))) (p : state) : dfa.evalFrom l p → (project m dfa).evalFrom (l.map (fun f => remove_index m f)) ⟨[p], by exact List.nodup_singleton p⟩ := by
+theorem evalFrom_project [DecidableEq state](dfa : DFA (Fin (n + 1) → Fin (b+2)) state) (m : Fin (n + 1)) (l : List (Fin (n+1) → Fin (b+2))) (p : state) : dfa.evalFrom l p → (project m dfa).evalFrom (l.map (fun f => remove_index m f)) ⟨[p], by exact List.nodup_singleton p⟩ := by
   simp[NFA.evalFrom, DFAO.evalFrom]
   intro h
   use (DFAO.transFrom dfa l p)
   constructor
-  . apply project_transFrom
+  . apply transFrom_project
     rfl
   . simp only [project]
     exact h
 
-theorem project_eval [DecidableEq state](dfa : DFA (Fin (n + 1) → Fin (b+2)) state) (m : Fin (n + 1)) (l : List (Fin (n+1) → Fin (b+2))) : dfa.eval l → (project m dfa).eval (l.map (fun f => remove_index m f)) := by
+theorem eval_project [DecidableEq state](dfa : DFA (Fin (n + 1) → Fin (b+2)) state) (m : Fin (n + 1)) (l : List (Fin (n+1) → Fin (b+2))) : dfa.eval l → (project m dfa).eval (l.map (fun f => remove_index m f)) := by
   simp[NFA.eval, DFAO.eval]
-  exact project_evalFrom dfa m l dfa.start
+  exact evalFrom_project dfa m l dfa.start
+
+-- theorem project_transition' [DecidableEq state](dfa : DFA (Fin (n + 1) → Fin (b+2)) state) (m : Fin (n + 1)) (f : (Fin n → Fin (b+2))) (p q : state) : q ∈ ((project m dfa).transition f p).val → ∃ f₁, f = remove_index m f₁ ∧ dfa.transition f₁ p = q := by
+--   simp only [project, List.mem_dedup, List.mem_map, FinEnum.mem_toList, true_and]
+--   intro h
+--   rcases h with ⟨a, h'⟩
+--   use recover_value m a f
+--   constructor
+--   . simp only [recover_value, remove_insert]
+--   . exact h'
+
+theorem project_transition [DecidableEq state](dfa : DFA (Fin (n + 1) → Fin (b+2)) state) (m : Fin (n + 1)) (f : (Fin n → Fin (b+2))) (p q : state) : q ∈ ((project m dfa).transition f p).val → ∃ a, dfa.transition (recover_value m a f) p = q := by
+  simp only [project, List.mem_dedup, List.mem_map, FinEnum.mem_toList, true_and, imp_self]
+
+theorem project_transFrom [DecidableEq state](dfa : DFA (Fin (n + 1) → Fin (b+2)) state) (m : Fin (n + 1)) (l : List (Fin n → Fin (b+2))) (q : state) (states : ListND state) : q ∈ ((project m dfa).transFrom l states).val → ∃ p ∈ states.val, ∃ (l₁ : List (Fin (n+1) → Fin (b+2))) , l = l₁.map (remove_index m) ∧ dfa.transFrom l₁ p = q:= by
+  intro h
+  induction l generalizing states
+  case nil =>
+    simp only [NFA.transFrom, List.mem_singleton] at h
+    simp_all only [List.nil_eq, List.map_eq_nil, exists_eq_left]
+    use q
+    simp only [h, DFAO.transFrom, and_self]
+  case cons f fs ih =>
+    simp [NFA.transFrom] at h
+    specialize ih ((project m dfa).transList f states)
+    specialize ih h
+    rcases ih with ⟨p, h₁, l₁, h₂, h₃⟩
+    -- Need to obtain a p' ∈ states.val from h₁. so p ∈ NFA.transList implies exists p', p  is in transitions.
+    have h₄ := NFA.transList_backtrack (project m dfa) f p states h₁
+    rcases h₄ with ⟨p', h₅, h₆⟩
+    use p'
+    constructor
+    . exact h₅
+    . have h₇ := project_transition dfa m f p' p h₆
+      rcases h₇ with ⟨a, h₈⟩
+      use (recover_value m a f) :: l₁
+      constructor
+      . simp only [recover_value, List.map_cons, remove_insert, List.cons.injEq, true_and]
+        simp only [h₂, remove_index]
+      . aesop
+
+theorem project_evalFrom [DecidableEq state](dfa : DFA (Fin (n + 1) → Fin (b+2)) state) (m : Fin (n + 1)) (l : List (Fin n → Fin (b+2))) (states : ListND state) : (project m dfa).evalFrom l states → ∃ p ∈ states.val, ∃ (l₁ : List (Fin (n+1) → Fin (b+2))) , l = l₁.map (remove_index m) ∧ dfa.evalFrom l₁ p:= by
+  intro h
+  simp_all [NFA.evalFrom, DFAO.evalFrom]
+  rcases h with ⟨p, h₁, h₂⟩
+  have h₃ := project_transFrom dfa m l p states h₁
+  rcases h₃ with ⟨p', h₄, h₅, h₆, h₇⟩
+  use p'
+  constructor
+  . exact h₄
+  . use h₅
+    constructor
+    . exact h₆
+    . simp only [project] at h₂
+      simp only [h₇, h₂]
+
+theorem project_eval [DecidableEq state](dfa : DFA (Fin (n + 1) → Fin (b+2)) state) (m : Fin (n + 1)) (l : List (Fin n → Fin (b+2))) : (project m dfa).eval l → ∃ (l₁ : List (Fin (n+1) → Fin (b+2))) , l = l₁.map (remove_index m) ∧ dfa.eval l₁ := by
+  simp[NFA.eval, DFAO.eval]
+  have h := project_evalFrom dfa m l (project m dfa).start
+  intro h₁
+  specialize h h₁
+  rcases h with ⟨p, h₂, l', h₄⟩
+  simp[project] at h₂
+
+  aesop?
+
+theorem project_eval_iff [DecidableEq state](dfa : DFA (Fin (n + 1) → Fin (b+2)) state) (m : Fin (n + 1)) (l : List (Fin n → Fin (b+2))) : (project m dfa).eval l ↔ ∃ (l₁ : List (Fin (n+1) → Fin (b+2))) , l = l₁.map (remove_index m) ∧ dfa.eval l₁ := by
+  constructor
+  . exact project_eval dfa m l
+  . intro h
+    rcases h with ⟨l₁, h₁, h₂⟩
+    have h₃ := eval_project dfa m l₁ h₂
+    aesop
 
 
-theorem project_acceptZero [DecidableEq state] (dfa : DFA (Fin (n + 1) → Fin (b+2)) state) (h: DFA.respectZero dfa) (m : Fin (n + 1)) : NFA.acceptZero (project m dfa) := by
+theorem project_acceptZero [DecidableEq state] (dfa : DFA (Fin (n + 1) → Fin (b+2)) state) (h: DFA.acceptZero dfa) (m : Fin (n + 1)) : NFA.acceptZero (project m dfa) := by
+  simp[NFA.acceptZero]
+  intro l h'
+  have h₁ := project_eval_iff dfa m l
+  have h₂ := h₁.mp h'
+  rcases h₂ with ⟨l₁, h₃, h₄⟩
+  rw[DFA.acceptZero] at h
+  specialize h l₁ h₄
+  intro k
+  specialize h k
+  have h₅ := project_eval_iff dfa m (padZeroes k l)
+  apply h₅.mpr
+  use (padZeroes k l₁)
+  constructor
+  . simp only [padZeroes, List.map_append, List.map_replicate]
+    have: List.replicate k (remove_index m (fun _ ↦ 0 : Fin (n+1) → Fin (b+2))) ++ List.map (remove_index m) l₁ = List.replicate k (fun _ ↦ 0) ++ List.map (remove_index m) l₁ := by
+      simp only [List.append_cancel_right_eq, List.replicate_inj, true_and]
+      right
+      simp only [remove_index]
+      ext x
+      simp only [Fin.removeNth, Fin.val_zero]
+    simp only [h₃, this]
+  . exact h
+
+theorem project_fix_respectZero [Fintype state][DecidableEq state] (dfa : DFA (Fin (n + 1) → Fin (b+2)) state) (m : Fin (n + 1)) (h: dfa.respectZero) : (project m dfa).fixLeadingZeros.respectZero := by
   sorry
 
 theorem project_correct [Fintype state] [DecidableEq state] (l : List ℕ) (hl : l.length = len)(m : Fin (len + 1)) (dfa : DFA (Fin (len +1) → Fin (b+2)) state) (h: dfa.acceptZero):
